relalg.v
@@ -17,25 +17,25 @@ Unset Printing Implicit Defensive.
 
 (** generic lemmas *)
 
-Lemma dottx `{laws} `{TOP<<l} n m (x: X n m): x ≦ top⋅x.
+Lemma dottx `{laws} `{TOP ≪ l} n m (x: X n m): x ≦ top⋅x.
 Proof. rewrite <-dot1x at 1. apply dot_leq; lattice. Qed.
 
-Lemma dotxt `{laws} `{TOP<<l} n m (x: X m n): x ≦ x⋅top.
+Lemma dotxt `{laws} `{TOP ≪ l} n m (x: X m n): x ≦ x⋅top.
 Proof. dual @dottx. Qed.
 
-Lemma top_nnm `{laws} `{TOP<<l} n m: top' n n ⋅ top' n m ≡ top' n m. 
+Lemma top_nnm `{laws} `{TOP ≪ l} n m: top' n n ⋅ top' n m ≡ top' n m. 
 Proof. apply leq_tx_iff. apply dottx. Qed.
 
-Lemma top_mnn `{laws} `{TOP<<l} n m: top' m n ⋅ top' n n ≡ top' m n. 
+Lemma top_mnn `{laws} `{TOP ≪ l} n m: top' m n ⋅ top' n n ≡ top' m n. 
 Proof. dual @top_nnm. Qed.
 
-Lemma disjoint_id `{laws} `{AL+BOT<<l} n m (p q: X n m): p ⊓ q ≦ 0 -> 1 ⊓ (p⋅q°) ≡ 0. 
+Lemma disjoint_id `{laws} `{AL+BOT ≪ l} n m (p q: X n m): p ⊓ q ≦ 0 -> 1 ⊓ (p⋅q°) ≡ 0. 
 Proof. 
   intro Hpq. apply leq_xb_iff. rewrite capC, capxdot. ra_normalise.
   rewrite Hpq. ra. 
 Qed.
 
-Lemma dedekind `{laws} `{AL<<l} n m p (x : X n m) (y : X m p) (z : X n p):
+Lemma dedekind `{laws} `{AL ≪ l} n m p (x : X n m) (y : X m p) (z : X n p):
   x⋅y ⊓ z ≦ (x ⊓ (z⋅y°))⋅(y ⊓ (x°⋅z)).
 Proof. rewrite <-(capI z) at 1. rewrite capA, capdotx, capxdot. ra. Qed.
   
@@ -50,10 +50,10 @@ Ltac tc := solve [eauto with typeclass_instances].
 Class is_nonempty {X: ops} n m (x: X n m) := nonempty: forall p q, top' p q ≦ top ⋅ x ⋅ top.
 Notation is_nonempty' m := (is_nonempty (one m)).
 
-Lemma nonempty_dom `{laws} `{TOP<<l} n m {x: X n m} {Hx: is_nonempty x}: is_nonempty' n.
+Lemma nonempty_dom `{laws} `{TOP ≪ l} n m {x: X n m} {Hx: is_nonempty x}: is_nonempty' n.
 Proof. intros i j. rewrite nonempty. mrewrite (leq_xt (x⋅top' _ j)). ra. Qed.
 
-Lemma nonempty_cod `{laws} `{TOP<<l} n m {x: X n m} {Hx: is_nonempty x}: is_nonempty' m.
+Lemma nonempty_cod `{laws} `{TOP ≪ l} n m {x: X n m} {Hx: is_nonempty x}: is_nonempty' m.
 Proof. intros i j. rewrite nonempty. rewrite (leq_xt (top' i _⋅x)). ra. Qed.
 
 
@@ -105,23 +105,23 @@ Context {L: laws l X}.
 
 Global Instance is_reflexive_weq {n}: Proper (weq ==> iff) (@is_reflexive n).
 Proof. intros ? ? E. unfold is_reflexive. now rewrite E. Qed.
-Global Instance is_irreflexive_weq {n} `{CAP<<l}: Proper (weq ==> iff) (@is_irreflexive n).
+Global Instance is_irreflexive_weq {n} `{CAP ≪ l}: Proper (weq ==> iff) (@is_irreflexive n).
 Proof. intros ? ? E. unfold is_irreflexive. now rewrite E. Qed.
 Global Instance is_transitive_weq {n}: Proper (weq ==> iff) (@is_transitive n).
 Proof. intros ? ? E. unfold is_transitive. now rewrite E. Qed.
-Global Instance is_linear_weq `{CUP+CNV<<l} {n}: Proper (weq ==> iff) (@is_linear n).
+Global Instance is_linear_weq `{CUP+CNV ≪ l} {n}: Proper (weq ==> iff) (@is_linear n).
 Proof. intros ? ? E. unfold is_linear. now rewrite E. Qed.
-Global Instance is_symmetric_weq `{CNV<<l} {n}: Proper (weq ==> iff) (@is_symmetric n).
+Global Instance is_symmetric_weq `{CNV ≪ l} {n}: Proper (weq ==> iff) (@is_symmetric n).
 Proof. intros ? ? E. unfold is_symmetric. now rewrite E. Qed.
-Global Instance is_antisymmetric_weq `{AL<<l} {n}: Proper (weq ==> iff) (@is_antisymmetric n).
+Global Instance is_antisymmetric_weq `{AL ≪ l} {n}: Proper (weq ==> iff) (@is_antisymmetric n).
 Proof. intros ? ? E. unfold is_antisymmetric. now rewrite E. Qed.
-Global Instance is_univalent_weq `{CNV<<l} {n m}: Proper (weq ==> iff) (@is_univalent n m).
+Global Instance is_univalent_weq `{CNV ≪ l} {n m}: Proper (weq ==> iff) (@is_univalent n m).
 Proof. intros ? ? E. unfold is_univalent. now rewrite E. Qed.
-Global Instance is_injective_weq `{CNV<<l} {n m}: Proper (weq ==> iff) (@is_injective n m).
+Global Instance is_injective_weq `{CNV ≪ l} {n m}: Proper (weq ==> iff) (@is_injective n m).
 Proof. intros ? ? E. unfold is_injective. now rewrite E. Qed.
-Global Instance is_surjective_weq `{CNV<<l} {n m}: Proper (weq ==> iff) (@is_surjective n m).
+Global Instance is_surjective_weq `{CNV ≪ l} {n m}: Proper (weq ==> iff) (@is_surjective n m).
 Proof. intros ? ? E. unfold is_surjective. now rewrite E. Qed.
-Global Instance is_total_weq `{CNV<<l} {n m}: Proper (weq ==> iff) (@is_total n m).
+Global Instance is_total_weq `{CNV ≪ l} {n m}: Proper (weq ==> iff) (@is_total n m).
 Proof. intros ? ? E. unfold is_total. now rewrite E. Qed.
 Global Instance is_vector_weq {n m}: Proper (weq ==> iff) (@is_vector n m).
 Proof. intros ? ? E. unfold is_vector. now rewrite E. Qed.
@@ -131,28 +131,28 @@ Proof. intros ? ? E. unfold is_nonempty. now setoid_rewrite E. Qed.
 Lemma proper_weq_leq_iff n m (P: X n m -> Prop): Proper (weq ==> impl) P -> Proper (weq ==> iff) P.
 Proof. intros HP ? ? E. split; now apply HP. Qed.
 
-Global Instance is_point_weq `{CNV<<l} {n m}: Proper (weq ==> iff) (@is_point n m).
+Global Instance is_point_weq `{CNV ≪ l} {n m}: Proper (weq ==> iff) (@is_point n m).
 Proof. apply proper_weq_leq_iff. intros ? ? E [? ? ?]. split; now rewrite <-E. Qed.
-Global Instance is_atom_weq `{CNV<<l} {n m}: Proper (weq ==> iff) (@is_atom n m).
+Global Instance is_atom_weq `{CNV ≪ l} {n m}: Proper (weq ==> iff) (@is_atom n m).
 Proof. apply proper_weq_leq_iff. intros ? ? E [? ? ?]. split; now rewrite <-E. Qed.
-Global Instance is_mapping_weq `{CNV<<l} {n m}: Proper (weq ==> iff) (@is_mapping n m).
+Global Instance is_mapping_weq `{CNV ≪ l} {n m}: Proper (weq ==> iff) (@is_mapping n m).
 Proof. apply proper_weq_leq_iff. intros ? ? E [? ?]. split; now rewrite <-E. Qed.
-Global Instance is_per_weq `{CNV<<l} {n}: Proper (weq ==> iff) (@is_per n).
+Global Instance is_per_weq `{CNV ≪ l} {n}: Proper (weq ==> iff) (@is_per n).
 Proof. apply proper_weq_leq_iff. intros ? ? E [? ?]. split; now rewrite <-E. Qed.
 Global Instance is_preorder_weq {n}: Proper (weq ==> iff) (@is_preorder n).
 Proof. apply proper_weq_leq_iff. intros ? ? E [? ?]. split; now rewrite <-E. Qed.
-Global Instance is_order_weq `{AL<<l} {n}: Proper (weq ==> iff) (@is_order n).
+Global Instance is_order_weq `{AL ≪ l} {n}: Proper (weq ==> iff) (@is_order n).
 Proof. apply proper_weq_leq_iff. intros ? ? E [? ?]. split; now rewrite <-E. Qed.
 
 (** alternative characterisation of [is_surjective] *)
 
-Lemma surjective_tx `{TOP<<l} {n m} {x: X n m} {Hx: is_surjective x} p: top' p _ ⋅ x ≡ top.
+Lemma surjective_tx `{TOP ≪ l} {n m} {x: X n m} {Hx: is_surjective x} p: top' p _ ⋅ x ≡ top.
 Proof.
   apply leq_tx_iff. transitivity (top' p _ ⋅ (x° ⋅ x)).
   rewrite <-surjective. ra. rewrite dotA. apply dot_leq; lattice.
 Qed.
 
-Lemma tx_surjective `{AL+TOP<<l} n m (x: X m n): top' n n ≦ top⋅x -> is_surjective x.
+Lemma tx_surjective `{AL+TOP ≪ l} n m (x: X m n): top' n n ≦ top⋅x -> is_surjective x.
 Proof.
   intro E. unfold is_surjective.
   transitivity (1 ∩ (top' n m ⋅ x)). rewrite <-E. lattice.
@@ -161,67 +161,67 @@ Qed.
 
 (** basic properties  *)
 
-Lemma symmetric `{CNV<<l} {n} {x: X n n} {Hx: is_symmetric x}: x° ≡ x.
+Lemma symmetric `{CNV ≪ l} {n} {x: X n n} {Hx: is_symmetric x}: x° ≡ x.
 Proof. apply antisym. assumption. now cnv_switch. Qed.
 
-Lemma irreflexive' `{BL<<l} {n} {x: X n n} {Hx: is_irreflexive x}: x ≦ !1.
+Lemma irreflexive' `{BL ≪ l} {n} {x: X n n} {Hx: is_irreflexive x}: x ≦ !1.
 Proof. now rewrite <-leq_cap_neg', Hx. Qed.
 
-Lemma vector' `{TOP<<l} {n m} {v: X n m} {Hv: is_vector v} x: v ⋅ x ≦ v.
+Lemma vector' `{TOP ≪ l} {n m} {v: X n m} {Hv: is_vector v} x: v ⋅ x ≦ v.
 Proof. rewrite <-vector at 2. ra. Qed.
 
-Lemma top_nonempty `{TOP<<l} {n m p} {Hm: is_nonempty' m}: top' n m ⋅ top' m p ≡ top.
+Lemma top_nonempty `{TOP ≪ l} {n m p} {Hm: is_nonempty' m}: top' n m ⋅ top' m p ≡ top.
 Proof. apply leq_tx_iff. rewrite nonempty. ra. Qed.
 
 
 (** instances for proof search  *)
 
-Global Instance point_surjective `{AL+TOP<<l} {n m} {p: X n m} {Hp: is_point p}: is_surjective p | 1.
+Global Instance point_surjective `{AL+TOP ≪ l} {n m} {p: X n m} {Hp: is_point p}: is_surjective p | 1.
 Proof. apply tx_surjective. rewrite nonempty at 1. now mrewrite vector. Qed.
 
-Global Instance atom_injective `{TOP<<l} {n m} {a: X n m} {Ha: is_atom a}: is_injective a.
+Global Instance atom_injective `{TOP ≪ l} {n m} {a: X n m} {Ha: is_atom a}: is_injective a.
 Proof. unfold is_injective. rewrite <-a_top_a'. rewrite <-(leq_xt 1). ra. Qed.
 
-Global Instance atom_univalent `{TOP<<l} {n m} {a: X n m} {Ha: is_atom a}: is_univalent a.
+Global Instance atom_univalent `{TOP ≪ l} {n m} {a: X n m} {Ha: is_atom a}: is_univalent a.
 Proof. unfold is_univalent. rewrite <-a'_top_a. rewrite <-(leq_xt 1). ra. Qed.
 
-Global Instance is_symmetric_neg1 `{BL+CNV<<l} {n}: is_symmetric (!one n).
+Global Instance is_symmetric_neg1 `{BL+CNV ≪ l} {n}: is_symmetric (!one n).
 Proof. unfold is_symmetric. rewrite <-dotx1. apply Schroeder_. rewrite negneg. ra. Qed.
 
-Global Instance irreflexive_cnv `{AL+BOT<<l} {n} {x: X n n} {H: is_irreflexive x}: is_irreflexive (x°).
+Global Instance irreflexive_cnv `{AL+BOT ≪ l} {n} {x: X n n} {H: is_irreflexive x}: is_irreflexive (x°).
 Proof. unfold is_irreflexive. cnv_switch. now ra_normalise. Qed.
 
-Global Instance reflexive_cnv `{CNV<<l} {n} {x: X n n} {H: is_reflexive x}: is_reflexive (x°).
+Global Instance reflexive_cnv `{CNV ≪ l} {n} {x: X n n} {H: is_reflexive x}: is_reflexive (x°).
 Proof. unfold is_reflexive. cnv_switch. now ra_normalise. Qed.
 
-Global Instance transitive_cnv `{CNV<<l} {n} {x: X n n} {H: is_transitive x}: is_transitive (x°).
+Global Instance transitive_cnv `{CNV ≪ l} {n} {x: X n n} {H: is_transitive x}: is_transitive (x°).
 Proof. unfold is_transitive. cnv_switch. now ra_normalise. Qed.
 
-Global Instance symmetric_cnv `{CNV<<l} {n} {x: X n n} {H: is_symmetric x}: is_symmetric (x°).
+Global Instance symmetric_cnv `{CNV ≪ l} {n} {x: X n n} {H: is_symmetric x}: is_symmetric (x°).
 Proof. unfold is_symmetric. now cnv_switch. Qed.
 
-Global Instance antisymmetric_cnv `{AL<<l} {n} {x: X n n} {H: is_antisymmetric x}: is_antisymmetric (x°).
+Global Instance antisymmetric_cnv `{AL ≪ l} {n} {x: X n n} {H: is_antisymmetric x}: is_antisymmetric (x°).
 Proof. unfold is_antisymmetric. now rewrite cnv_invol, capC. Qed.
 
-Global Instance injective_cnv `{CNV<<l} {n m} {x: X n m} {H: is_univalent x}: is_injective (x°).
+Global Instance injective_cnv `{CNV ≪ l} {n m} {x: X n m} {H: is_univalent x}: is_injective (x°).
 Proof. unfold is_injective. now rewrite cnv_invol. Qed.
 
-Global Instance univalent_cnv `{CNV<<l} {n m} {x: X n m} {H: is_injective x}: is_univalent (x°).
+Global Instance univalent_cnv `{CNV ≪ l} {n m} {x: X n m} {H: is_injective x}: is_univalent (x°).
 Proof. unfold is_univalent. now rewrite cnv_invol. Qed.
 
-Global Instance surjective_cnv `{CNV<<l} {n m} {x: X n m} {H: is_total x}: is_surjective (x°).
+Global Instance surjective_cnv `{CNV ≪ l} {n m} {x: X n m} {H: is_total x}: is_surjective (x°).
 Proof. unfold is_surjective. now rewrite cnv_invol. Qed.
 
-Global Instance total_cnv `{CNV<<l} {n m} {x: X n m} {H: is_surjective x}: is_total (x°).
+Global Instance total_cnv `{CNV ≪ l} {n m} {x: X n m} {H: is_surjective x}: is_total (x°).
 Proof. unfold is_total. now rewrite cnv_invol. Qed.
 
-Global Instance preorder_cnv `{CNV<<l} {n} {x: X n n} {H: is_preorder x}: is_preorder (x°).
+Global Instance preorder_cnv `{CNV ≪ l} {n} {x: X n n} {H: is_preorder x}: is_preorder (x°).
 Proof. constructor; tc. Qed.
 
-Global Instance nonempty_cnv `{CNV+TOP<<l} {n m} {x: X n m} {Hx: is_nonempty x}: is_nonempty (x°).
+Global Instance nonempty_cnv `{CNV+TOP ≪ l} {n m} {x: X n m} {Hx: is_nonempty x}: is_nonempty (x°).
 Proof. intros i j. cnv_switch. ra_normalise. apply Hx. Qed.
 
-Global Instance atom_cnv `{CNV+TOP<<l} {n m} {x: X n m} {Hx: is_atom x}: is_atom (x°).
+Global Instance atom_cnv `{CNV+TOP ≪ l} {n m} {x: X n m} {Hx: is_atom x}: is_atom (x°).
 Proof.
   split.
   rewrite cnv_invol. apply a'_top_a.
@@ -229,43 +229,43 @@ Proof.
   apply nonempty_cnv.
 Qed.
 
-Global Instance mapping_cnv `{AL+TOP<<l} {n m} {x: X n m} {Hx: is_point x}: is_mapping (x°).
+Global Instance mapping_cnv `{AL+TOP ≪ l} {n m} {x: X n m} {Hx: is_point x}: is_mapping (x°).
 Proof. split; tc. Qed.          (* actually just need x to be injective and surjective *)
 
-Global Instance order_cnv `{AL<<l} {n} {x: X n n} {Hx: is_order x}: is_order (x°).
+Global Instance order_cnv `{AL ≪ l} {n} {x: X n n} {Hx: is_order x}: is_order (x°).
 Proof. constructor; tc. Qed.
 
-Global Instance vector_cap `{CAP+TOP<<l} {n m} {v w: X n m} {Hv: is_vector v} {Hw: is_vector w}: is_vector (v ⊓ w). 
+Global Instance vector_cap `{CAP+TOP ≪ l} {n m} {v w: X n m} {Hv: is_vector v} {Hw: is_vector w}: is_vector (v ⊓ w). 
 Proof. 
   unfold is_vector. apply antisym. 2: apply dotxt. 
   now rewrite dotcapx, 2vector. 
 Qed.   
 
-Global Instance preorder_str `{STR<<l} n (x: X n n): is_preorder (x^*).
+Global Instance preorder_str `{STR ≪ l} n (x: X n n): is_preorder (x^*).
 Proof. split. apply str_refl. apply weq_leq, str_trans. Qed.
 
-Global Instance symmetric_str `{STR+CNV<<l} {n} {x: X n n} {Hx: is_symmetric x}: is_symmetric (x^*).
+Global Instance symmetric_str `{STR+CNV ≪ l} {n} {x: X n n} {Hx: is_symmetric x}: is_symmetric (x^*).
 Proof. unfold is_symmetric. now rewrite cnvstr, symmetric. Qed.
 
-Global Instance reflexive_itr `{STR<<l} {n} {x: X n n} {Hx: is_reflexive x}: is_reflexive (x^+).
+Global Instance reflexive_itr `{STR ≪ l} {n} {x: X n n} {Hx: is_reflexive x}: is_reflexive (x^+).
 Proof. unfold is_reflexive. rewrite reflexive. apply itr_ext. Qed.
 
-Global Instance transitive_itr `{STR<<l} n (x: X n n): is_transitive (x^+).
+Global Instance transitive_itr `{STR ≪ l} n (x: X n n): is_transitive (x^+).
 Proof. apply itr_trans. Qed.
 
-Global Instance symmetric_itr `{STR+CNV<<l} {n} {x: X n n} {Hx: is_symmetric x}: is_symmetric (x^+).
+Global Instance symmetric_itr `{STR+CNV ≪ l} {n} {x: X n n} {Hx: is_symmetric x}: is_symmetric (x^+).
 Proof. unfold is_symmetric. now rewrite cnvitr, symmetric. Qed.
 
 
 (** lemmas about relations of a specific shape *)
 
-Lemma itr_transitive `{STR<<l} n (x: X n n): is_transitive x -> x^+ ≡ x.
+Lemma itr_transitive `{STR ≪ l} n (x: X n n): is_transitive x -> x^+ ≡ x.
 Proof. intro. apply antisym. now apply itr_ind_l1. apply itr_ext. Qed.
 
-Lemma str_transitive `{KA<<l} n (x: X n n): is_transitive x -> x^* ≡ 1+x.
+Lemma str_transitive `{KA ≪ l} n (x: X n n): is_transitive x -> x^* ≡ 1+x.
 Proof. intro. now rewrite str_itr, itr_transitive. Qed.
 
-Lemma dot_mono `{AL<<l} n (x y: X n n): x ≦ 1 -> y ≦ 1 -> x⋅y ≡ x ⊓ y. 
+Lemma dot_mono `{AL ≪ l} n (x y: X n n): x ≦ 1 -> y ≦ 1 -> x⋅y ≡ x ⊓ y. 
 Proof. 
   intros Hx Hy. apply antisym. apply leq_xcap.
    rewrite Hy; ra.
@@ -275,7 +275,7 @@ Proof.
   ra_normalise. apply dot_leq; lattice. 
 Qed.
 
-Lemma kernel_refl_antisym `{laws} `{CAP+CNV<<l} {n} {x: X n n}
+Lemma kernel_refl_antisym `{laws} `{CAP+CNV ≪ l} {n} {x: X n n}
   {Hr: is_reflexive x} {Ha: is_antisymmetric x}: x° ⊓ x ≡ 1. 
 Proof. 
   apply antisym. assumption.
@@ -283,11 +283,11 @@ Proof.
   now rewrite <-reflexive. 
 Qed. 
 
-Lemma dot_univalent_cap `{AL<<l} {n m p} {x: X n m} {y z: X m p}
+Lemma dot_univalent_cap `{AL ≪ l} {n m p} {x: X n m} {y z: X m p}
   {E: is_univalent x}: x ⋅ (y ∩ z) ≡ (x⋅y) ∩ (x⋅z).  
 Proof. apply antisym. ra. rewrite capdotx. mrewrite univalent. ra. Qed.
 
-Lemma univalent_antisym `{AL+TOP<<l} {n m} {x y: X n m}
+Lemma univalent_antisym `{AL+TOP ≪ l} {n m} {x y: X n m}
   {Hy: is_univalent y}: y⋅top' m m ≦ x⋅top -> x ≦ y -> x ≡ y. 
 Proof. 
   intros Ht Hxy. apply antisym. assumption.
@@ -296,7 +296,7 @@ Proof.
   ra_normalise. rewrite Hxy at 2. mrewrite univalent. ra.
 Qed.
 
-Lemma surjective_injective_antisym `{AL+TOP<<l} {n m} {p q: X n m}
+Lemma surjective_injective_antisym `{AL+TOP ≪ l} {n m} {p q: X n m}
    {Hp: is_surjective p} {Hq: is_injective q}: p ≦ q -> p ≡ q. 
 Proof.
   intros Hpq. cnv_switch. apply univalent_antisym.
@@ -304,14 +304,14 @@ Proof.
   now cnv_switch.
 Qed.
 
-Lemma disjoint_vect_iff `{BL+CNV<<l} {n m} {p q: X n m}
+Lemma disjoint_vect_iff `{BL+CNV ≪ l} {n m} {p q: X n m}
   {Hq: is_vector q}: p ⊓ q ≦ 0 <-> q°⋅p ≦ 0.
 Proof.
   rewrite Schroeder_l, cnv_invol, negbot.
   rewrite vector, capC. apply leq_cap_neg'.
 Qed.
 
-Lemma disjoint_vect_iff' `{AL+DIV+BOT+TOP<<l} {n m} {p q: X n m}
+Lemma disjoint_vect_iff' `{AL+DIV+BOT+TOP ≪ l} {n m} {p q: X n m}
   {Hq: is_vector q}: p ⊓ q ≦ 0 <-> q°⋅p ≦ 0.
 Proof.
   split; intro Hpq.
@@ -320,7 +320,7 @@ Proof.
   rewrite <-vector at 1. rewrite capdotx. rewrite ldv_cancel. ra.
 Qed.
 
-Lemma gen_point {Hl: CNV+TOP<<l} n m k (p: X n m):
+Lemma gen_point {Hl: CNV+TOP ≪ l} n m k (p: X n m):
    is_nonempty' k -> is_point p -> is_point (p⋅top' m k).
 Proof.
   intros Hk Hp. split.
@@ -330,7 +330,7 @@ Proof.
   intros i j. mrewrite (top_nonempty (n:=m) (m:=k) (p:=j)). apply nonempty. 
 Qed.
 
-Lemma leq_xyp `{AL+TOP<<l} {n m k} {p: X m k} {x: X n k} {y: X n m}
+Lemma leq_xyp `{AL+TOP ≪ l} {n m k} {p: X m k} {x: X n k} {y: X n m}
   {Hp: is_point p}: x ≦ y⋅p <-> x⋅p° ≦ y.
 Proof.
   split; intro E.
@@ -338,11 +338,11 @@ Proof.
    rewrite <-(dotx1 x). rewrite surjective. now mrewrite E.
 Qed.
 
-Lemma leq_pxq `{AL+TOP<<l} {n m k} {p: X n k} {q: X m k} {x: X n m}
+Lemma leq_pxq `{AL+TOP ≪ l} {n m k} {p: X n k} {q: X m k} {x: X n m}
    {Hp: is_point p} {Hq: is_point q}: p ≦ x⋅q <-> q ≦x°⋅p.
 Proof. rewrite 2leq_xyp. now rewrite cnv_leq_iff', cnvdot, cnv_invol. Qed.
 
-Lemma point_lattice_atom {Hl: AL+TOP<<l} {n m} {p v: X n m} {Hp: is_point p} {Hv: is_vector v}:
+Lemma point_lattice_atom {Hl: AL+TOP ≪ l} {n m} {p v: X n m} {Hp: is_point p} {Hv: is_vector v}:
   is_nonempty v -> v ≦ p -> v ≡ p.
 Proof.
   intros Hv' Hvp. apply antisym. assumption.
@@ -353,32 +353,32 @@ Proof.
 Qed.
 
 
-Lemma dot_neg_inj {Hl: BL+CNV<<l} {n m p} {x: X n m} {y: X m p} {Hy: is_injective y}: !x ⋅ y ≦ !(x⋅y).
+Lemma dot_neg_inj {Hl: BL+CNV ≪ l} {n m p} {x: X n m} {y: X m p} {Hy: is_injective y}: !x ⋅ y ≦ !(x⋅y).
 Proof. rewrite Schroeder_r, 2negneg. mrewrite injective. ra. Qed.
 
-Lemma dot_neg_surj {Hl: BL+CNV<<l} {n m p} {x: X n m} {y: X m p} {Hy: is_surjective y}: !(x⋅y) ≦ !x ⋅ y.
+Lemma dot_neg_surj {Hl: BL+CNV ≪ l} {n m p} {x: X n m} {y: X m p} {Hy: is_surjective y}: !(x⋅y) ≦ !x ⋅ y.
 Proof.
   rewrite leq_cap_neg. rewrite <-negcup, <-dotplsx, cupneg. now rewrite surjective_tx, negtop.
 Qed.
 
-Lemma dot_neg_point {Hl: BL+CNV<<l} {n m k} {x: X n m} {p: X m k} {Hp: is_point p}: !x ⋅ p ≡ !(x⋅p).
+Lemma dot_neg_point {Hl: BL+CNV ≪ l} {n m k} {x: X n m} {p: X m k} {Hp: is_point p}: !x ⋅ p ≡ !(x⋅p).
 Proof. apply antisym. apply dot_neg_inj. apply dot_neg_surj. Qed.
 
-Lemma disjoint_vect_ext {Hl: BL+CNV<<l} {n m k} {x y: X n m} {x' y': X m k}
+Lemma disjoint_vect_ext {Hl: BL+CNV ≪ l} {n m k} {x y: X n m} {x' y': X m k}
       {Hx: is_vector x}: x ⊓ y ≦ 0 -> (x ⋅ x') ⊓ (y ⋅ y') ≦ 0.
 Proof.
   rewrite capC. intro H. apply disjoint_vect_iff in H.
   rewrite capdotx. mrewrite H. ra.
 Qed.
 
-Lemma atom_of_points_aux `{AL+TOP<<l} {n m k} {p: X n m} {q: X k m} {Hp: is_point p} {Hq: is_point q}:
+Lemma atom_of_points_aux `{AL+TOP ≪ l} {n m k} {p: X n m} {q: X k m} {Hp: is_point p} {Hq: is_point q}:
   p ⋅ q° ⋅ top ⋅ q ⋅ p° ≦ 1.
 Proof.
   mrewrite surjective_tx. transitivity (p⋅(top⋅q)°⋅p°). ra.
   mrewrite surjective_tx. ra_normalise. rewrite vector. now apply injective.
 Qed.
 
-Lemma atom_of_points `{AL+TOP<<l} {n m k} {p: X n m} {q: X k m} {Hp: is_point p} {Hq: is_point q}:
+Lemma atom_of_points `{AL+TOP ≪ l} {n m k} {p: X n m} {q: X k m} {Hp: is_point p} {Hq: is_point q}:
   is_atom (p⋅q°).
 Proof.
   split. ra_normalise. apply atom_of_points_aux. 
@@ -386,7 +386,7 @@ Proof.
   intros i j. mrewrite (surjective_tx (x:=p)). now apply nonempty_cnv.
 Qed.
 
-Lemma point_a_top `{CNV+TOP<<l} {n m} {a: X n m} {Ha: is_atom a}: is_point (a⋅top' m m).
+Lemma point_a_top `{CNV+TOP ≪ l} {n m} {a: X n m} {Ha: is_atom a}: is_point (a⋅top' m m).
 Proof.
   split.
   unfold is_vector. now mrewrite top_nnm.
@@ -394,17 +394,17 @@ Proof.
   intros i j. mrewrite top_nnm. apply atom_nonempty.
 Qed.
 
-Lemma point_a'_top `{CNV+TOP<<l} {n m} {a: X n m} {Ha: is_atom a}: is_point (a°⋅top' n n).
+Lemma point_a'_top `{CNV+TOP ≪ l} {n m} {a: X n m} {Ha: is_atom a}: is_point (a°⋅top' n n).
 Proof. apply point_a_top. Qed.
 
-Lemma a_top_a_aux `{AL+TOP<<l} {n m} {a: X n m} {Ha: is_atom a}: (a ⋅ top) ∩ (top ⋅ a) ≡ a.
+Lemma a_top_a_aux `{AL+TOP ≪ l} {n m} {a: X n m} {Ha: is_atom a}: (a ⋅ top) ∩ (top ⋅ a) ≡ a.
 Proof.
   apply antisym.
   rewrite capdotx. mrewrite a'_top_a. ra.
   rewrite <-2(leq_xt 1). ra. 
 Qed.  
   
-Lemma a_top_a `{AL+TOP<<l} {n m} {a: X n m} {Ha: is_atom a}: a ⋅ top ⋅ a ≡ a.
+Lemma a_top_a `{AL+TOP ≪ l} {n m} {a: X n m} {Ha: is_atom a}: a ⋅ top ⋅ a ≡ a.
 Proof.
   rewrite <-a_top_a_aux at 3.
   apply antisym.
@@ -412,18 +412,18 @@ Proof.
   rewrite capdotx. mrewrite <-(leq_xt (a°⋅top' n n)). ra.
 Qed.
 
-Global Instance atom_transitive `{AL+TOP<<l} {n} {a: X n n} {Ha: is_atom a}: is_transitive a.
+Global Instance atom_transitive `{AL+TOP ≪ l} {n} {a: X n n} {Ha: is_atom a}: is_transitive a.
 Proof. unfold is_transitive. rewrite <-a_top_a at 3. rewrite <-(leq_xt 1). ra. Qed.
 
 (* TOTHINK: transitivity should follow from mono *)
-Lemma atom_mono `{AL+TOP<<l} {n} {a: X n n} {Ha: is_atom a}: a⋅a ≦ 1.
+Lemma atom_mono `{AL+TOP ≪ l} {n} {a: X n n} {Ha: is_atom a}: a⋅a ≦ 1.
 Proof.
   transitivity (a⋅a ⊓ a). apply leq_xcap. reflexivity. apply atom_transitive.
   rewrite dedekind. transitivity ((a⋅a°)⋅(a°⋅a)). apply dot_leq; lattice.
   mrewrite (injective (x:=a)). mrewrite (univalent (x:=a)). ra.
 Qed.
 
-Lemma atom_points `{AL+TOP<<l} {n m k} {a: X n m} {Ha: is_atom a} {Hk: is_nonempty' k}:
+Lemma atom_points `{AL+TOP ≪ l} {n m k} {a: X n m} {Ha: is_atom a} {Hk: is_nonempty' k}:
   exists p q: X _ k, is_point p /\ is_point q /\ a ≡ p⋅q°.
 Proof.
   exists (a⋅top). exists (a°⋅top). 
@@ -432,7 +432,7 @@ Proof.
   ra_normalise. mrewrite (top_nonempty (n:=m) (p:=n)). now rewrite a_top_a.
 Qed.
 
-Lemma atom_lattice_atom {Hl: AL+TOP<<l} {n m} {a x: X n m} {Ha: is_atom a}:
+Lemma atom_lattice_atom {Hl: AL+TOP ≪ l} {n m} {a x: X n m} {Ha: is_atom a}:
   is_nonempty x -> x ≦ a -> x ≡ a.
 Proof.
   intros Hx Hax. 
@@ -448,12 +448,12 @@ End props.
 
 (** lemmas obtained by duality *)
 
-Lemma total_xt `{laws} `{TOP<<l} {n m} {x: X n m} {Hx: is_total x} p: x⋅top' _ p ≡ top.
+Lemma total_xt `{laws} `{TOP ≪ l} {n m} {x: X n m} {Hx: is_total x} p: x⋅top' _ p ≡ top.
 Proof. now dual @surjective_tx. Qed.
 
-Lemma xt_total `{laws} `{AL+TOP<<l} n m (x: X n m): top' n n ≦ x⋅top -> is_total x.
+Lemma xt_total `{laws} `{AL+TOP ≪ l} n m (x: X n m): top' n n ≦ x⋅top -> is_total x.
 Proof. now dual @tx_surjective. Qed.
 
-Lemma dot_cap_injective `{laws} `{AL<<l} {n m p} {x: X m n} {y z: X p m}
+Lemma dot_cap_injective `{laws} `{AL ≪ l} {n m p} {x: X m n} {y z: X p m}
       {Hx: is_injective x}: (y ∩ z) ⋅ x ≡ (y⋅x) ∩ (z⋅x).  
 Proof. revert Hx. dual @dot_univalent_cap. Qed.
