rewriting.v
@@ -126,13 +126,13 @@ Require Export AAC.
 Section lattice.
 Context `{lattice.laws}. 
 
-Global Instance aac_cupA `{CUP<<l} : Associative weq cup := cupA.
-Global Instance aac_cupC `{CUP<<l} : Commutative weq cup := cupC.
-Global Instance aac_cupU `{BOT+CUP<<l} : Unit weq cup bot := Build_Unit _ _ _ cupbx cupxb.
+Global Instance aac_cupA `{CUP ≪ l} : Associative weq cup := cupA.
+Global Instance aac_cupC `{CUP ≪ l} : Commutative weq cup := cupC.
+Global Instance aac_cupU `{BOT+CUP ≪ l} : Unit weq cup bot := Build_Unit _ _ _ cupbx cupxb.
 
-Global Instance aac_capA `{CAP<<l} : Associative weq cap := capA.
-Global Instance aac_capC `{CAP<<l} : Commutative weq cap := capC.
-Global Instance aac_capU `{TOP+CAP<<l} : Unit weq cap top := Build_Unit _ _ _ captx capxt.
+Global Instance aac_capA `{CAP ≪ l} : Associative weq cap := capA.
+Global Instance aac_capC `{CAP ≪ l} : Commutative weq cap := capC.
+Global Instance aac_capU `{TOP+CAP ≪ l} : Unit weq cap top := Build_Unit _ _ _ captx capxt.
 
 Global Instance aac_lift_leq_weq : AAC_lift leq weq. 
 Proof. constructor; eauto with typeclass_instances. Qed.
@@ -150,7 +150,7 @@ End monoid.
 (* tests for AAC_tactics *)
 (*
 Require Import kleene.
-Goal forall `{laws} `{BKA<<l} n (a b c: X n n), a+b ≡ c -> (forall x: X n n, x⋅x ≡ x) -> 
+Goal forall `{laws} `{BKA ≪ l} n (a b c: X n n), a+b ≡ c -> (forall x: X n n, x⋅x ≡ x) -> 
   a⋅b+b+1⋅a+(b+0)^* ≡ a⋅b*c⋅b*c⋅a+0.
 Proof. 
   intros. aac_normalise. 
