sums.v
@@ -25,15 +25,15 @@ Notation "\sum_ ( i < n ) f" := (\sum_(i \in seq n) f)
     format "'[' \sum_ ( i < n ) '/  '  f ']'"): ra_terms.
 
 (** [dot] distributes over sums *)
-Lemma dotxsum `{laws} `{BSL<<l} I J n m p (f: I -> X m n) (x: X p m): 
+Lemma dotxsum `{laws} `{BSL ≪ l} I J n m p (f: I -> X m n) (x: X p m): 
   x ⋅ (\sum_(i\in J) f i) ≡ \sum_(i\in J) (x ⋅ f i).
 Proof. apply f_sup_weq. apply dotx0. intros; apply dotxpls. Qed.
 
-Lemma dotsumx `{laws} `{BSL<<l} I J n m p (f: I -> X n m) (x: X m p): 
+Lemma dotsumx `{laws} `{BSL ≪ l} I J n m p (f: I -> X n m) (x: X m p): 
   (\sum_(i\in J) f i) ⋅ x ≡ \sum_(i\in J) (f i ⋅ x).
 Proof. dual @dotxsum. Qed.
 
 (** converse commutes with sums *)
-Lemma cnvsum `{laws} `{BSL+CNV<<l} I J n m (f: I -> X n m): 
+Lemma cnvsum `{laws} `{BSL+CNV ≪ l} I J n m (f: I -> X n m): 
   (\sum_(i\in J) f i)° ≡ \sum_(i \in J) (f i)°.
 Proof. apply f_sup_weq. apply cnv0. apply cnvpls. Qed.
